Kami/Ex/ProcThreeStDec.v
@@ -17,9 +17,6 @@ Section ProcThreeStDec.
             (dec: AbsDec addrSize instBytes dataBytes rfIdx)
             (exec: AbsExec addrSize iaddrSize instBytes dataBytes rfIdx).
 
-  Variable predictNextPc: forall ty, fullType ty (SyntaxKind (Pc iaddrSize)) -> (* pc *)
-                                     Expr ty (SyntaxKind (Pc iaddrSize)).
-
   Variable (d2eElt: Kind).
   Variable (d2ePack:
               forall ty,
@@ -92,7 +89,7 @@ Section ProcThreeStDec.
   Variable (init: ProcInit iaddrSize dataBytes rfIdx).
 
   Definition p3st := ProcThreeStage.p3st
-                       fetch dec exec predictNextPc
+                       fetch dec exec
                        d2ePack d2eOpType d2eDst d2eAddr d2eVal1 d2eVal2
                        d2eRawInst d2eCurPc d2eNextPc d2eEpoch
                        e2wPack e2wDecInst e2wVal init.
@@ -213,7 +210,7 @@ Section ProcThreeStDec.
     kinv_red.
 
   Definition p3stInl := ProcThreeStInl.p3stInl
-                          fetch dec exec predictNextPc
+                          fetch dec exec
                           d2ePack d2eOpType d2eDst d2eAddr d2eVal1 d2eVal2
                           d2eRawInst d2eCurPc d2eNextPc d2eEpoch
                           e2wPack e2wDecInst e2wVal init.
