Kami/Ex/ProcThreeStInl.v
@@ -11,9 +11,6 @@ Section Inlined.
             (dec: AbsDec addrSize instBytes dataBytes rfIdx)
             (exec: AbsExec addrSize iaddrSize instBytes dataBytes rfIdx).
 
-  Variable predictNextPc: forall ty, fullType ty (SyntaxKind (Pc iaddrSize)) -> (* pc *)
-                                     Expr ty (SyntaxKind (Pc iaddrSize)).
-
   Variable (d2eElt: Kind).
   Variable (d2ePack:
               forall ty,
@@ -59,7 +56,7 @@ Section Inlined.
 
   Variable (init: ProcInit iaddrSize dataBytes rfIdx).
 
-  Definition p3st := p3st fetch dec exec predictNextPc
+  Definition p3st := p3st fetch dec exec
                           d2ePack d2eOpType d2eDst d2eAddr d2eVal1 d2eVal2
                           d2eRawInst d2eCurPc d2eNextPc d2eEpoch
                           e2wPack e2wDecInst e2wVal init.
